tests.lean
@@ -3,23 +3,26 @@ import decide
 open term
 def x := var 0
 def y := var 1
--- Checking I sub and neg and neg_one satisfy the defining identities
+
+-- Checking if the operations satisfy the defining identities
 #eval decide (x + -x) 0
+#eval decide (incr x) (x + 1)
+#eval decide (decr x) (x - 1)
 #eval decide (x + - y) (x - y)
 #eval decide (neg_one) (-1)
 #eval decide (x + 0) (var 0)
 #eval decide (x + y) (y + x)
 
 -- Equalities from Zulip
-#eval decide (-var 0) (not x + 1)
-#eval decide (-var 0) (not (x - 1))
-#eval decide (not x) (-x - 1)
-#eval decide (-not x) (x + 1)
-#eval decide (x + y) (x - not y + neg_one)
+#eval decide (-x) (not x).incr
+#eval decide (-x) (not x.decr)
+#eval decide (not x) (-x).decr
+#eval decide (-not x) x.incr
+#eval decide (x + y) (x - not y).decr
 #eval decide (x + y) ((xor x y) + (and x y).ls)
 #eval decide (x + y) (or x y + and x y)
 #eval decide (x + y) ((or x y).ls - (xor x y))
---#eval decide (x - y) (x + not y + 1)
+#eval decide (x - y) (x + not y).incr
 #eval decide (x - y) (xor x y - (and (not x) y).ls)
 #eval decide (x - y) (and x (not y) - (and (not x) y))
 #eval decide (x - y) ((and x (not y)).ls - (xor x y))
@@ -27,9 +30,9 @@ def y := var 1
 #eval decide (and x (not y)) (or x y - y)
 #eval decide (and x (not y)) (x - and x y)
 
-#eval decide (not (x - y)) (y - x + neg_one)
+#eval decide (not (x - y)) (y - x).decr
 #eval decide (not (x - y)) (not x + y)
-#eval decide (not (xor x y)) (and x y - or x y + neg_one)
+#eval decide (not (xor x y)) (and x y - (or x y)).decr
 #eval decide (not (xor x y)) (and x y + not (or x y))
 #eval decide (or x y) (and x (not y) + y)
 #eval decide (and x y) (or (not x) y - not x)
